Prove create with dir isolation
For simplicity require permission to modify entire subtree, but
technically only permissions on the directory itself and the file being
created are required, since no deeper files/directories are being
created.

src/DirectoryIsolatedFS.v
@@ -445,8 +445,8 @@ Qed.
 Ltac split_lifted_prop :=
   match goal with
   | [ H: _ (lower_disk (get vdisk _)) |- _ ] =>
-    repeat apply sep_star_assoc_2 in H;
-    apply sep_star_lift_apply in H;
+    (repeat apply sep_star_assoc_2 in H; apply sep_star_lift_apply in H)
+    || (apply sep_star_comm in H; apply sep_star_lift_apply in H);
     destruct_ands
   end.
 
@@ -584,6 +584,31 @@ Definition update_fblock_d1 inum off v :=
 Definition update_fblock_d inum off v :=
   fuel_retry (update_fblock_d1 inum off v).
 
+Definition create1 dnum name :=
+  fsxp <- Get mFsxp;
+    mscs <- Get mMscs;
+    r <- CFS.create fsxp dnum name mscs;
+    match r with
+    | Some r =>
+      let '(mscs', (r, _)) := r in
+      _ <- Assgn mMscs mscs';
+        _ <- ConcurrentCache.cache_commit;
+        _ <- match r with
+            | OK inum =>
+              let f' := DIRTREE.TreeFile inum BFILE.bfile0 in
+              let up := DIRTREE.add_to_dir name f' in
+              var_update vDirTree (DIRTREE.alter_inum dnum up)
+            | _ => Ret tt
+            end;
+        Ret (value r)
+    | None =>
+      _ <- ConcurrentCache.cache_abort;
+        Ret None
+    end.
+
+Definition create dnum name :=
+  fuel_retry (create1 dnum name).
+
 Ltac member_index_ne := match goal with
                         | |- member_index ?v1 <> member_index ?v2 =>
                           try unfold v1; try unfold v2;
@@ -678,6 +703,162 @@ Qed.
 
 Hint Resolve dirtree_rep_tree_names_distinct
      dirtree_rep_tree_inodes_distinct.
+
+Theorem create1_ok : forall dnum name,
+      SPEC App.delta, tid |-
+              {{ pathname tree_elem,
+               | PRE d hm m s_i s:
+                   let tree := get vDirTree s in
+                   invariant App.delta d hm m s /\
+                   DIRTREE.find_subtree pathname tree = Some (DIRTREE.TreeDir dnum tree_elem) /\
+                   (forall suffix, owner_le (Owned tid) (path_owner (get vPathOwner s) (pathname ++ suffix))) /\
+                   guar App.delta tid s_i s
+               | POST d' hm' m' s_i' s' r:
+                   let tree' := get vDirTree s' in
+                   invariant App.delta d' hm' m' s' /\
+                   match r with
+                   | Some (OK inum) =>
+                     let f' := DIRTREE.TreeFile inum BFILE.bfile0 in
+                     tree' = DIRTREE.tree_graft dnum tree_elem pathname name f'
+                                                (get vDirTree s)
+                   | _ => tree' = get vDirTree s
+                   end /\
+                   guar App.delta tid s s' /\
+                   hashmap_le hm hm' /\
+                   guar App.delta tid s_i' s'
+              }} create1 dnum name.
+Proof.
+  unfold create1, wrap_syscall; intros.
+  step.
+  step.
+  step.
+
+  match goal with
+  | [ H: invariant App.delta _ _ _ _ |- _ ] =>
+    simpl in H
+  end.
+  match goal with
+  | [ H: guar App.delta _ _ _ |- _ ] =>
+    simpl in H
+  end.
+  destruct_ands; repeat deex.
+  (* exists_tuple breaks apart ds *)
+  destruct ds.
+
+  unfold project_disk.
+  repeat eapply exists_tuple; eexists; simpl.
+  intuition eauto.
+
+  replace (get vdisk s).
+  pred_apply; cancel; eauto.
+
+  step.
+  destruct matches; subst.
+  - step.
+    step.
+    unfold cacheI in *; simpl_get_set_all; intuition eauto.
+    step.
+    step.
+    unfold cacheI in *; simpl_get_set_all;
+      rewrite ?get_set_other in * by member_index_ne;
+      intuition eauto.
+    repeat match goal with
+           | [ H: get _ _ = get _ _ |- _ ] => rewrite H
+           end.
+    match goal with
+    | [ H: (emp * _)%pred (lower_disk (get vdisk s0)) |- _ ] =>
+      apply star_emp_pimpl in H
+    end; repeat split_lifted_prop.
+    unfold or in *; (intuition idtac); repeat split_lifted_prop;
+      try match goal with
+          | [ H: isError (OK _) |- _] =>
+            exfalso; inversion H
+          end.
+    unfold exis in *; repeat (deex || split_lifted_prop).
+    subst.
+
+    descend; intuition idtac.
+    pred_apply; cancel.
+    pred_apply; cancel.
+
+    unfold dirtree_alter_file.
+    erewrite DIRTREE.alter_inum_to_alter_path by eauto.
+    erewrite dirtree_alter_to_update by eauto.
+    cancel.
+
+    repeat match goal with
+           | [ H: get _ _ = get _ _ |- _ ] => rewrite H
+           end.
+    unfold dirtree_alter_file.
+    erewrite DIRTREE.alter_inum_to_alter_path by eauto.
+    erewrite dirtree_alter_to_update by eauto.
+    eauto.
+
+    eapply cacheR_preorder; eauto.
+    eapply cacheR_preorder; eauto.
+    unfold cacheR; rewrite ?get_set_other by member_index_ne; try reflexivity.
+
+    repeat match goal with
+           | [ H: get _ _ = get _ _ |- _ ] => rewrite H
+           end.
+    replace (get vPathOwner s_i).
+    unfold dirtree_alter_file.
+    erewrite DIRTREE.alter_inum_to_alter_path by eauto.
+    erewrite dirtree_alter_to_update by eauto.
+
+    eapply allowed_subtree_update; eauto.
+
+    eapply cacheR_preorder; eauto.
+    eapply cacheR_preorder; eauto.
+    eapply cacheR_preorder; eauto.
+    unfold cacheR; rewrite ?get_set_other by member_index_ne; try reflexivity.
+
+    eapply allowed_preorder; eauto.
+    repeat match goal with
+           | [ H: get _ _ = get _ _ |- _ ] => rewrite H
+           end.
+    replace (get vPathOwner s_i).
+    unfold dirtree_alter_file.
+    erewrite DIRTREE.alter_inum_to_alter_path by eauto.
+    erewrite dirtree_alter_to_update by eauto.
+    eapply allowed_subtree_update; eauto.
+  - step.
+    step.
+
+    unfold cacheI; simpl_get_set_all; intuition eauto.
+
+    step.
+
+    repeat match goal with
+           | [ H: get _ _ = get _ _ |- _ ] => rewrite H
+           end.
+    descend; intuition eauto.
+    pred_apply; cancel.
+    eapply cacheR_preorder; eauto.
+    eapply cacheR_preorder; eauto.
+    eapply cacheR_preorder; eauto.
+
+    etransitivity; eauto.
+    replace (get vDirTree s).
+    replace (get vDirTree s0).
+    reflexivity.
+  - step.
+    step.
+
+    repeat match goal with
+           | [ H: get _ _ = get _ _ |- _ ] => rewrite H
+           end.
+    descend; intuition eauto.
+
+    eapply cacheR_preorder; eauto.
+    eapply cacheR_preorder; eauto.
+    eapply cacheR_preorder; eauto.
+
+    etransitivity; eauto.
+    replace (get vDirTree s).
+    replace (get vDirTree s0).
+    reflexivity.
+Qed.
 
 Theorem update_fblock_d1_ok : forall inum off v,
       SPEC App.delta, tid |-
@@ -1872,11 +2053,6 @@ Definition tree_sync :=
                      (* this is a complete spec - tree sync does not affect the
                 latest tree *)
                      (fun tree => tree).
-
-Definition create dnum name :=
-  wrap_syscall_loop (fun fsxp mscs =>
-                       CFS.create fsxp dnum name mscs)
-                    (fun tree => tree).
 
 Definition rename dnum srcpath srcname dstpath dstname :=
   wrap_syscall_loop (fun fsxp mscs =>
